Added some additional derived rules for word theory manipulations, in particular BIT_WORD_CONV, for explicit expressions for bits of a word operation (including recursive ones for operations with carries like word_add and word_sub), e.g.
  # BIT_WORD_CONV `bit 7 (word_or x y:int16)`;;
  val it : thm = |- bit 7 (word_or x y) <=> bit 7 x \/ bit 7 y

and WORD_RED_CONV / WORD_REDUCE_CONV to do general explicit computations
by proof with expressions of the form "word n" for concrete numeral n and
concrete word size, e.g.

  # WORD_REDUCE_CONV `word_xor (word 255:byte) (word 252:byte)`;;
  val it : thm = |- word_xor (word 255) (word 252) = word 3

Also added a few additional word operations with results that are
at least debatable or really vary among common ISAs (e.g. how to treat
shifts bigger than the word size, how to do truncating division with
negative numbers). These are broadly intended to match JVM behaviour
and so are tagged with the letter j even in cases where they don't
precisely correspond to JVM operations:

        word_jdiv
        word_jrem
        word_jrol
        word_jror
        word_jshl
        word_jshr
        word_jushr

and also added a few simple theorems about those new concepts:

        IVAL_TOPFLIP_VAL
        VAL_WORD_NEG_MOD_DIMINDEX
        WORD_JROL
        WORD_JROL_JROR
        WORD_JROR
        WORD_JROR_JROL
        WORD_UGE_TOPFLIP
        WORD_UGT_TOPFLIP
        WORD_ULE_TOPFLIP
        WORD_ULT_TOPFLIP

Finally added a few more trivial integer theorems

        INT_GCD_EQ
        INT_MUL_DIV_EQ
        INT_REM_2_CASES
        INT_REM_2_DIVIDES
        NOT_INT_REM_2

as well as renaming the theorem INT_DIVISION_DECOMP in "int.ml" to
INT_DIVISION_SIMP, which better maintains the pattern of DIVISION_SIMP
and avoids a clash with a different theorem in "Library/integer.ml".

Library/words.ml
@@ -15,6 +15,13 @@
 (* and unsigned variants (e.g. `word_ushr` is unsigned/logical shift right,  *)
 (* while `word_ishr` is signed/arithmetical shift right).                    *)
 (*                                                                           *)
+(* For some cases where the result is debatable or machine-dependent, we     *)
+(* have versions that match the JVM tagged with a "j" (e.g. `word_jshr`      *)
+(* truncates shift counts modulo word size).                                 *)
+(*                                                                           *)
+(* There are conversions like WORD_REDUCE_CONV for reducing via proof        *)
+(* expressions built up from concrete words like `word 255:byte`.            *)
+(*                                                                           *)
 (* Some simple decision procedures for proving basic equalities are here too *)
 (* and have limited and somewhat complementary scopes:                       *)
 (*  - WORD_RULE for simple algebraic properties                              *)
@@ -2832,3 +2839,1366 @@ let WORD_BITMASK = prove
   REWRITE_TAC[WORD_OF_BITS_MASK; WORD_OF_BITS_SING_AS_WORD] THEN
   REWRITE_TAC[WORD_SUB; ARITH_RULE `1 <= n <=> ~(n = 0)`] THEN
   REWRITE_TAC[EXP_EQ_0; ARITH_EQ]);;
+
+(* ------------------------------------------------------------------------- *)
+(* JVM-specific word operations, though they may well work in other places.  *)
+(*                                                                           *)
+(* All shift operations mask out the lower bits as the unsigned shift count. *)
+(*                                                                           *)
+(* Division does truncation towards zero; at this level there is no concept  *)
+(* of an exception on division by zero. Note that the JVM is defined anyway  *)
+(* so INT_MIN / -1 doesn't generate any exception, just returning the        *)
+(* correct modular result as per the usual pattern.                          *)
+(*                                                                           *)
+(* Remainder is then defined by the usual Euclidean identity.                *)
+(* ------------------------------------------------------------------------- *)
+
+let word_jshl = new_definition
+ `word_jshl (x:N word) (y:N word) =
+        word_shl x (val y MOD dimindex(:N))`;;
+
+let word_jshr = new_definition
+ `word_jshr (x:N word) (y:N word) =
+        word_ishr x (val y MOD dimindex(:N))`;;
+
+let word_jushr = new_definition
+ `word_jushr (x:N word) (y:N word) =
+        word_ushr x (val y MOD dimindex(:N))`;;
+
+let word_jdiv = new_definition
+ `word_jdiv:N word->N word->N word =
+   imodular (\a b. int_sgn a * int_sgn b * (abs(a) div abs(b)))`;;
+
+let word_jrem = new_definition
+ `word_jrem (x:N word) (y:N word) =
+    word_sub x (word_mul (word_jdiv x y) y)`;;
+
+(* ------------------------------------------------------------------------- *)
+(* The JVM doesn't include rotates as primitive, but here is what they       *)
+(* obviously would be like, and proof that some emulations work. Note that   *)
+(* emulation using negative shifts relies not only on the Java               *)
+(* masking treatment of shift counts but also on the word size being a       *)
+(* power of 2 (of course for the JVM it is 2^5 = 32 or 2^6 = 64).            *)
+(* ------------------------------------------------------------------------- *)
+
+let word_jror = new_definition
+ `word_jror (w:N word) (k:N word) = word_ror w (val k)`;;
+
+let word_jrol = new_definition
+ `word_jrol (w:N word) (k:N word) = word_rol w (val k)`;;
+
+let VAL_WORD_NEG_MOD_DIMINDEX = prove
+ (`!k:N word.
+        dimindex(:N) divides 2 EXP dimindex(:N)
+        ==> (val(word_neg k) == dimindex (:N) - val k MOD dimindex(:N))
+            (mod dimindex(:N))`,
+  REPEAT STRIP_TAC THEN REWRITE_TAC[VAL_WORD_NEG; CONG] THEN
+  MATCH_MP_TAC(MESON[]
+   `x MOD n MOD m = x MOD m /\ x MOD m = y ==> x MOD n MOD m = y`) THEN
+  CONJ_TAC THENL [ASM_MESON_TAC[divides; MOD_MOD]; ALL_TAC] THEN
+  REWRITE_TAC[GSYM CONG; num_congruent] THEN
+  SIMP_TAC[GSYM INT_OF_NUM_SUB; LT_IMP_LE; VAL_BOUND; DIVISION;
+           DIMINDEX_NONZERO; GSYM INT_OF_NUM_REM] THEN
+  MATCH_MP_TAC(INTEGER_RULE
+   `n divides e /\ (k':int == k) (mod n) ==> (e - k == n - k') (mod n)`) THEN
+  ASM_REWRITE_TAC[GSYM num_divides; INT_REM_MOD_SELF]);;
+
+let WORD_JROL_JROR = prove
+ (`!w k:N word.
+        dimindex(:N) divides 2 EXP dimindex(:N)
+        ==> word_jrol w k = word_jror w (word_neg k)`,
+  REPEAT STRIP_TAC THEN REWRITE_TAC[word_jrol; word_jror] THEN
+  REWRITE_TAC[WORD_ROL_ROR_GEN] THEN MATCH_MP_TAC WORD_ROR_PERIODIC THEN
+  ONCE_REWRITE_TAC[NUMBER_RULE
+   `(x:num == y) (mod n) <=> (y == x) (mod n)`] THEN
+  MATCH_MP_TAC VAL_WORD_NEG_MOD_DIMINDEX THEN ASM_REWRITE_TAC[]);;
+
+let WORD_JROR_JROL = prove
+ (`!w k:N word.
+        dimindex(:N) divides 2 EXP dimindex(:N)
+        ==> word_jror w k = word_jrol w (word_neg k)`,
+  REPEAT STRIP_TAC THEN REWRITE_TAC[word_jrol; word_jror] THEN
+  REWRITE_TAC[WORD_ROR_ROL_GEN] THEN MATCH_MP_TAC WORD_ROL_PERIODIC THEN
+  ONCE_REWRITE_TAC[NUMBER_RULE
+   `(x:num == y) (mod n) <=> (y == x) (mod n)`] THEN
+  MATCH_MP_TAC VAL_WORD_NEG_MOD_DIMINDEX THEN ASM_REWRITE_TAC[]);;
+
+let WORD_JROR = prove
+ (`!w k:N word.
+        dimindex(:N) divides 2 EXP dimindex(:N)
+        ==> word_jror w k =
+            word_or (word_jushr w k) (word_jshl w (word_neg k))`,
+  REPEAT STRIP_TAC THEN REWRITE_TAC[word_jror; word_jushr; word_jshl] THEN
+  ONCE_REWRITE_TAC[WORD_ROR_MOD] THEN
+  SIMP_TAC[WORD_ROR_SHIFTS; DIVISION; DIMINDEX_NONZERO; LT_IMP_LE] THEN
+  FIRST_X_ASSUM(MP_TAC o ISPEC `k:N word` o
+    MATCH_MP VAL_WORD_NEG_MOD_DIMINDEX) THEN
+  REWRITE_TAC[CONG] THEN DISCH_THEN SUBST1_TAC THEN
+  ASM_CASES_TAC `val(k:N word) MOD dimindex(:N) = 0` THENL
+   [ASM_REWRITE_TAC[SUB_0; MOD_REFL; WORD_USHR_ZERO; WORD_SHL_ZERO] THEN
+    MATCH_MP_TAC(WORD_BITWISE_RULE
+     `y = word 0 ==> word_or x y = word_or x x`) THEN
+    REWRITE_TAC[GSYM VAL_EQ_0; VAL_WORD_SHL; MOD_MULT];
+    AP_TERM_TAC THEN AP_TERM_TAC THEN
+    CONV_TAC SYM_CONV THEN MATCH_MP_TAC MOD_LT THEN
+    REWRITE_TAC[ARITH_RULE `n - k < n <=> ~(k = 0) /\ ~(n = 0)`] THEN
+    ASM_REWRITE_TAC[DIMINDEX_NONZERO]]);;
+
+let WORD_JROL = prove
+ (`!w k:N word.
+        dimindex(:N) divides 2 EXP dimindex(:N)
+        ==> word_jrol w k =
+            word_or (word_jshl w k) (word_jushr w (word_neg k))`,
+  REPEAT STRIP_TAC THEN ASM_SIMP_TAC[WORD_JROL_JROR; WORD_JROR] THEN
+  ONCE_REWRITE_TAC[WORD_RULE `word_neg(word_neg x):N word = x`] THEN
+  CONV_TAC WORD_BITWISE_RULE);;
+
+(* ------------------------------------------------------------------------- *)
+(* Conversion for "j" forms applied to numeral shift/rotate word.            *)
+(* ------------------------------------------------------------------------- *)
+
+let WORD_WORD_OPERATION_CONV =
+  let pth = prove
+   (`word_jshl (x:N word) (word n) =
+     word_shl x (n MOD (2 EXP dimindex(:N)) MOD dimindex(:N)) /\
+     word_jshr x (word n) =
+     word_ishr x (n MOD (2 EXP dimindex(:N)) MOD dimindex(:N)) /\
+     word_jushr x (word n) =
+     word_ushr x (n MOD (2 EXP dimindex(:N)) MOD dimindex(:N)) /\
+     word_jrol x (word n) =
+     word_rol x (n MOD (2 EXP dimindex(:N)) MOD dimindex(:N)) /\
+     word_jror x (word n) =
+     word_ror x (n MOD (2 EXP dimindex(:N)) MOD dimindex(:N))`,
+    REWRITE_TAC[word_jshl; word_jshr; word_jushr; word_jrol; word_jror] THEN
+    REWRITE_TAC[VAL_WORD; GSYM WORD_ROL_MOD; GSYM WORD_ROR_MOD]) in
+  GEN_REWRITE_CONV I [pth] THENC
+  RAND_CONV
+   (BINOP2_CONV (RAND_CONV (!word_POW2SIZE_CONV) THENC NUM_MOD_CONV)
+                (!word_SIZE_CONV) THENC
+    NUM_MOD_CONV);;
+
+(* ------------------------------------------------------------------------- *)
+(* Emulation of unsigned comparisons using signed (useful for the JVM).      *)
+(* ------------------------------------------------------------------------- *)
+
+let IVAL_TOPFLIP_VAL = prove
+ (`!w:N word.
+        ival(word_xor word_INT_MIN w) =
+        &(val w) - &2 pow (dimindex(:N) - 1)`,
+  REWRITE_TAC[INT_IVAL; WORD_XOR_INT_MIN] THEN
+  REWRITE_TAC[INT_VAL_WORD_ADD_CASES; INT_VAL_WORD_INT_MIN; MSB_INT_VAL] THEN
+  WORD_ARITH_TAC);;
+
+let WORD_ULE_TOPFLIP = prove
+ (`!v w:N word.
+        word_ule v w <=>
+        word_ile (word_xor (word_INT_MIN) v) (word_xor (word_INT_MIN) w)`,
+  REWRITE_TAC[word_ule; word_ile; relational2; irelational2] THEN
+  REWRITE_TAC[IVAL_TOPFLIP_VAL; GSYM INT_OF_NUM_LE] THEN INT_ARITH_TAC);;
+
+let WORD_ULT_TOPFLIP = prove
+ (`!v w:N word.
+        word_ult v w <=>
+        word_ilt (word_xor (word_INT_MIN) v) (word_xor (word_INT_MIN) w)`,
+  REWRITE_TAC[word_ult; word_ilt; relational2; irelational2] THEN
+  REWRITE_TAC[IVAL_TOPFLIP_VAL; GSYM INT_OF_NUM_LT] THEN INT_ARITH_TAC);;
+
+let WORD_UGE_TOPFLIP = prove
+ (`!v w:N word.
+        word_uge v w <=>
+        word_ige (word_xor (word_INT_MIN) v) (word_xor (word_INT_MIN) w)`,
+  REWRITE_TAC[word_uge; word_ige; relational2; irelational2] THEN
+  REWRITE_TAC[IVAL_TOPFLIP_VAL; INT_GE; GE; GSYM INT_OF_NUM_LE] THEN
+  INT_ARITH_TAC);;
+
+let WORD_UGT_TOPFLIP = prove
+ (`!v w:N word.
+        word_ugt v w <=>
+        word_igt (word_xor (word_INT_MIN) v) (word_xor (word_INT_MIN) w)`,
+  REWRITE_TAC[word_ugt; word_igt; relational2; irelational2] THEN
+  REWRITE_TAC[IVAL_TOPFLIP_VAL; INT_GT; GT; GSYM INT_OF_NUM_LT] THEN
+  INT_ARITH_TAC);;
+
+(* ------------------------------------------------------------------------- *)
+(* Conversion for explicit numeric bits of word operations, one level.       *)
+(* For example BIT_WORD_CONV `bit 7 (word_sub x y:int16)`                    *)
+(* ------------------------------------------------------------------------- *)
+
+let BIT_WORD_CONV =
+  let pth_ror = prove
+   (`bit i (word_ror (w:N word) n) <=>
+          (\m. (\s. if s < dimindex(:N) then bit s w
+                    else i < dimindex(:N) /\ bit (s - dimindex(:N)) w)
+               (i + m))
+          (n MOD dimindex(:N))`,
+    REWRITE_TAC[BIT_WORD_ROR])
+  and pth_rol = prove
+   (`bit i (word_rol (w:N word) n) <=>
+          (\m. if i < m then bit (i + dimindex(:N) - m) w
+               else i < dimindex(:N) /\ bit (i - m) w)
+          (n MOD dimindex(:N))`,
+    REWRITE_TAC[BIT_WORD_ROL]) in
+  let rule_add = (MATCH_MP o prove)
+   (`n = SUC m
+     ==> (bit n (word_add x y:N word) <=>
+          n < dimindex(:N) /\
+          ((bit n x <=> bit n y) <=>
+           bit m x /\ bit m y \/
+           (bit m x \/ bit m y) /\ ~bit m (word_add x y)))`,
+    SIMP_TAC[REWRITE_RULE[GSYM ADD1] BIT_WORD_ADD_CLAUSES])
+  and rule_sub = (MATCH_MP o prove)
+   (`n = SUC m
+     ==> (bit n (word_sub x y:N word) <=>
+          n < dimindex(:N) /\
+          ((bit n x <=> bit n y) <=>
+           ~bit m x /\ bit m y \/
+           (~bit m x \/ bit m y) /\ bit m (word_sub x y)))`,
+    SIMP_TAC[REWRITE_RULE[GSYM ADD1] BIT_WORD_SUB_CLAUSES])
+  and rule_neg = (MATCH_MP o prove)
+   (`n = SUC m
+     ==> (bit n (word_neg x:N word) <=>
+          n < dimindex(:N) /\
+          (bit n x <=> ~bit m x /\ ~bit m (word_neg x)))`,
+    SIMP_TAC[REWRITE_RULE[GSYM ADD1] BIT_WORD_NEG_CLAUSES])
+  and conv_shl = GEN_REWRITE_CONV I [REWRITE_RULE[CONJ_ASSOC] BIT_WORD_SHL]
+  and conv_ror = GEN_REWRITE_CONV I [pth_ror]
+  and conv_rol = GEN_REWRITE_CONV I [pth_rol]
+  and conv_cond_t = GEN_REWRITE_CONV I [CONJUNCT1(SPEC_ALL COND_CLAUSES)]
+  and conv_cond_f = GEN_REWRITE_CONV I [CONJUNCT2(SPEC_ALL COND_CLAUSES)]
+  and conv_and = GEN_REWRITE_CONV I [AND_CLAUSES]
+  and conv_and_t = GEN_REWRITE_CONV I [CONJUNCT1(SPEC_ALL AND_CLAUSES)]
+  and conv_and_f = GEN_REWRITE_CONV I [el 2 (CONJUNCTS(SPEC_ALL AND_CLAUSES))]
+  and zero_tm = `0` and one_tm = `1` in
+  fun tm ->
+    match tm with
+      Comb(Comb(Const("bit",_),n),Comb(Const("word",_),m))
+      when is_numeral n && is_numeral m ->
+          if m = zero_tm then
+            GEN_REWRITE_CONV I [BIT_WORD_0] tm
+          else if m = one_tm then
+            (GEN_REWRITE_CONV I [BIT_WORD_1] THENC NUM_EQ_CONV) tm
+          else
+            (GEN_REWRITE_CONV I [BIT_WORD] THENC
+             BINOP2_CONV (RAND_CONV(!word_SIZE_CONV) THENC NUM_LT_CONV)
+                         (RAND_CONV (RAND_CONV NUM_EXP_CONV THENC
+                                     NUM_DIV_CONV) THENC
+                          NUM_ODD_CONV) THENC
+             conv_and) tm
+    | Comb(Comb(Const("bit",_),n),Comb(Const("word",_),m))
+      when is_numeral n && m = one_tm ->
+          (GEN_REWRITE_CONV I [BIT_WORD_1] THENC NUM_EQ_CONV) tm
+    | Comb(Comb(Const("bit",_),n),Comb(Const("word_not",_),_))
+      when is_numeral n ->
+       (GEN_REWRITE_CONV I [BIT_WORD_NOT] THENC
+        LAND_CONV(RAND_CONV(!word_SIZE_CONV) THENC NUM_LT_CONV) THENC
+        conv_and) tm
+    | Comb(Comb(Const("bit",_),n),Comb(Comb(Const("word_and",_),_),_))
+      when is_numeral n ->
+        GEN_REWRITE_CONV I [BIT_WORD_AND_ALT] tm
+    | Comb(Comb(Const("bit",_),n),Comb(Comb(Const("word_or",_),_),_))
+      when is_numeral n ->
+        GEN_REWRITE_CONV I [BIT_WORD_OR_ALT] tm
+    | Comb(Comb(Const("bit",_),n),Comb(Comb(Const("word_xor",_),_),_))
+      when is_numeral n ->
+        GEN_REWRITE_CONV I [BIT_WORD_XOR_ALT] tm
+    | Comb(Comb(Const("bit",_),n),Comb(Comb(Const("word_add",_),_),_))
+      when is_numeral n ->
+        if n = zero_tm then
+         (GEN_REWRITE_CONV I [CONJUNCT1 BIT_WORD_ADD_CLAUSES]) tm
+        else
+         (GEN_REWRITE_CONV I [rule_add (num_CONV n)] THENC
+          LAND_CONV(RAND_CONV(!word_SIZE_CONV) THENC NUM_LT_CONV) THENC
+          conv_and) tm
+    | Comb(Comb(Const("bit",_),n),Comb(Comb(Const("word_sub",_),_),_))
+      when is_numeral n ->
+        if n = zero_tm then
+         (GEN_REWRITE_CONV I [CONJUNCT1 BIT_WORD_SUB_CLAUSES]) tm
+        else
+         (GEN_REWRITE_CONV I [rule_sub (num_CONV n)] THENC
+          LAND_CONV(RAND_CONV(!word_SIZE_CONV) THENC NUM_LT_CONV) THENC
+          conv_and) tm
+    | Comb(Comb(Const("bit",_),n),Comb(Const("word_neg",_),_))
+      when is_numeral n ->
+        if n = zero_tm then
+         (GEN_REWRITE_CONV I [CONJUNCT1 BIT_WORD_NEG_CLAUSES]) tm
+        else
+         (GEN_REWRITE_CONV I [rule_neg (num_CONV n)] THENC
+          LAND_CONV(RAND_CONV(!word_SIZE_CONV) THENC NUM_LT_CONV) THENC
+          conv_and) tm
+    | Comb(Comb(Const("bit",_),n),Comb(Comb(Const("word_shl",_),_),m))
+      when is_numeral n && is_numeral m ->
+        (conv_shl THENC
+         BINOP2_CONV (BINOP2_CONV NUM_LE_CONV
+                       (RAND_CONV(!word_SIZE_CONV) THENC NUM_LT_CONV) THENC
+                         conv_and)
+                     (LAND_CONV NUM_SUB_CONV) THENC
+         conv_and) tm
+    | Comb(Comb(Const("bit",_),n),Comb(Comb(Const("word_ushr",_),_),m))
+      when is_numeral n && is_numeral m ->
+        (GEN_REWRITE_CONV I [BIT_WORD_USHR] THENC LAND_CONV NUM_ADD_CONV) tm
+    | Comb(Comb(Const("bit",_),n),Comb(Comb(Const("word_ishr",_),_),m))
+      when is_numeral n && is_numeral m ->
+        (GEN_REWRITE_CONV I [BIT_WORD_ISHR] THENC
+         RATOR_CONV(LAND_CONV
+           (BINOP2_CONV NUM_ADD_CONV (!word_SIZE_CONV) THENC
+            NUM_LT_CONV)) THENC
+         ((conv_cond_t THENC
+           LAND_CONV NUM_ADD_CONV) ORELSEC
+          (conv_cond_f THENC
+           COMB2_CONV
+              (RAND_CONV(RAND_CONV(!word_SIZE_CONV) THENC NUM_LT_CONV))
+              (LAND_CONV(LAND_CONV(!word_SIZE_CONV) THENC NUM_SUB_CONV)) THENC
+           conv_and))) tm
+    | Comb(Comb(Const("bit",_),n),Comb(Comb(Const("word_ror",_),_),m))
+      when is_numeral n && is_numeral m ->
+        (conv_ror THENC
+         RAND_CONV (RAND_CONV(!word_SIZE_CONV) THENC NUM_MOD_CONV) THENC
+         BETA_CONV THENC RAND_CONV NUM_ADD_CONV THENC BETA_CONV THENC
+         RATOR_CONV(LAND_CONV
+          (RAND_CONV(!word_SIZE_CONV) THENC NUM_LT_CONV)) THENC
+         (conv_cond_t ORELSEC
+          (conv_cond_f THENC
+           LAND_CONV(RAND_CONV(!word_SIZE_CONV) THENC NUM_LT_CONV) THENC
+           ((conv_and_t THENC
+             LAND_CONV(RAND_CONV(!word_SIZE_CONV) THENC NUM_SUB_CONV)) ORELSEC
+            conv_and_f
+           ))))
+        tm
+    | Comb(Comb(Const("bit",_),n),Comb(Comb(Const("word_rol",_),_),m))
+      when is_numeral n && is_numeral m ->
+        (conv_rol THENC
+         RAND_CONV (RAND_CONV(!word_SIZE_CONV) THENC NUM_MOD_CONV) THENC
+         BETA_CONV THENC
+         RATOR_CONV(LAND_CONV NUM_LT_CONV) THENC
+         ((conv_cond_t THENC
+           LAND_CONV(RAND_CONV
+            (LAND_CONV(!word_SIZE_CONV) THENC NUM_SUB_CONV) THENC
+           NUM_ADD_CONV)) ORELSEC
+          (conv_cond_f THENC
+           LAND_CONV(RAND_CONV(!word_SIZE_CONV) THENC NUM_LT_CONV) THENC
+           ((conv_and_t THENC
+             LAND_CONV NUM_SUB_CONV) ORELSEC
+            conv_and_f)
+         ))) tm
+    | Comb(Comb(Const("bit",_),n),Comb(Comb(Const("word_join",_),_),_))
+      when is_numeral n ->
+        (GEN_REWRITE_CONV I [BIT_WORD_JOIN] THENC
+         LAND_CONV (RAND_CONV(!word_SIZE_CONV) THENC NUM_LT_CONV) THENC
+         (conv_and_f ORELSEC
+          (conv_and_t THENC
+           RATOR_CONV(LAND_CONV
+            (RAND_CONV(!word_SIZE_CONV) THENC NUM_LT_CONV)) THENC
+           (conv_cond_t ORELSEC
+            (conv_cond_f THENC
+             LAND_CONV(RAND_CONV(!word_SIZE_CONV) THENC NUM_SUB_CONV))
+          ))))
+        tm
+    | Comb(Comb(Const("bit",_),n),
+           Comb(Comb(Const("word_subword",_),_),
+                Comb(Comb(Const(",",_),p),q)))
+        when is_numeral n && is_numeral p && is_numeral q ->
+         (GEN_REWRITE_CONV I [BIT_WORD_SUBWORD] THENC
+          LAND_CONV
+           (RAND_CONV(RAND_CONV(!word_SIZE_CONV) THENC NUM_MIN_CONV) THENC
+            NUM_LT_CONV) THENC
+          ((conv_and_t THENC
+             LAND_CONV NUM_ADD_CONV) ORELSEC
+            conv_and_f)) tm
+    | _ -> failwith "BIT_WORD_CONV";;
+
+(* ------------------------------------------------------------------------- *)
+(* Conversions for explicit calculations with terms of the form "word n"     *)
+(* where n is a numeral. They all work for arbitrary n and whenever they     *)
+(* return "word m", then that will be canonical, i.e. m < 2^wordsize.        *)
+(* ------------------------------------------------------------------------- *)
+
+let WORD_WORD_CONV =
+  let pth = prove
+   (`word n:N word = word(n MOD (2 EXP dimindex(:N)))`,
+    REWRITE_TAC[WORD_MOD_SIZE]) in
+  fun tm ->
+    match tm with
+      Comb(Const("word",_),t) when is_numeral t ->
+        (GEN_REWRITE_CONV I [pth] THENC
+         funpow 2 RAND_CONV (!word_POW2SIZE_CONV) THENC
+         RAND_CONV NUM_MOD_CONV) tm
+    | _ -> failwith "WORD_WORD_CONV";;
+
+let WORD_IWORD_CONV tm =
+  match tm with
+   Comb(Const("iword",_),t) when is_intconst t ->
+     (REWR_CONV iword THENC
+      funpow 4 RAND_CONV (!word_SIZE_CONV) THENC
+      funpow 3 RAND_CONV INT_POW_CONV THENC
+      funpow 2 RAND_CONV INT_REM_CONV THENC
+      GEN_REWRITE_CONV RAND_CONV [NUM_OF_INT_OF_NUM]) tm
+  | _ -> failwith "WORD_IWORD_CONV";;
+
+let WORD_VAL_CONV tm =
+  match tm with
+    Comb(Const("val",_),Comb(Const("word",_),n)) when is_numeral n ->
+     (GEN_REWRITE_CONV I [VAL_WORD] THENC
+      funpow 2 RAND_CONV (!word_SIZE_CONV) THENC
+      RAND_CONV NUM_EXP_CONV THENC NUM_MOD_CONV) tm
+  | _ -> failwith "WORD_VAL_CONV";;
+
+let WORD_IVAL_CONV =
+  let pth = prove
+   (`ival(word n:N word) =
+        (\v. if v < 2 EXP (dimindex (:N) - 1)
+             then &v else &v - &2 pow dimindex(:N))
+        (val(word n:N word))`,
+    REWRITE_TAC[ival])
+  and cth1,cth2 = CONJ_PAIR
+   (MESON[] `(if T then x:int else y:int) = x /\
+             (if F then x:int else y:int) = y`) in
+  fun tm ->
+   (match tm with
+      Comb(Const("ival",_),Comb(Const("word",_),n)) when is_numeral n ->
+     (GEN_REWRITE_CONV I [pth] THENC
+      RAND_CONV WORD_VAL_CONV THENC
+      BETA_CONV THENC
+      RATOR_CONV(LAND_CONV
+       (RAND_CONV (RAND_CONV
+           (LAND_CONV (!word_SIZE_CONV) THENC NUM_SUB_CONV) THENC
+         NUM_EXP_CONV) THENC
+        NUM_LT_CONV)) THENC
+      (GEN_REWRITE_CONV I [cth1] ORELSEC
+       (GEN_REWRITE_CONV I [cth2] THENC
+        (RAND_CONV o RAND_CONV) (!word_SIZE_CONV) THENC
+        RAND_CONV INT_POW_CONV THENC INT_SUB_CONV))) tm
+    | _ -> failwith "WORD_IVAL_CONV");;
+
+let WORD_BIT_CONV =
+  let pth0 = prove
+   (`(ODD(0 DIV 2 EXP k) <=> F) /\
+     (ODD(NUMERAL(BIT0 n) DIV 2 EXP 0) <=> F) /\
+     (ODD(NUMERAL(BIT1 n) DIV 2 EXP 0) <=> T)`,
+    REWRITE_TAC[DIV_0; ODD; EXP; DIV_1] THEN
+    REWRITE_TAC[NUMERAL; BIT0; BIT1] THEN
+    REWRITE_TAC[ODD; ODD_ADD])
+  and pth1 = prove
+   (`(ODD(NUMERAL(BIT0 n) DIV 2 EXP SUC k) <=> ODD(NUMERAL n DIV (2 EXP k))) /\
+     (ODD(NUMERAL(BIT1 n) DIV 2 EXP SUC k) <=> ODD(NUMERAL n DIV (2 EXP k)))`,
+    CONJ_TAC THEN AP_TERM_TAC THEN
+    GEN_REWRITE_TAC (BINOP_CONV o LAND_CONV) [NUMERAL] THEN
+    GEN_REWRITE_TAC (LAND_CONV o LAND_CONV) [BIT0; BIT1] THEN
+    REWRITE_TAC[EXP; GSYM DIV_DIV] THEN
+    AP_THM_TAC THEN AP_TERM_TAC THEN ARITH_TAC) in
+  let conv0 = GEN_REWRITE_CONV I [pth0]
+  and conv1 = GEN_REWRITE_CONV I [pth1]
+  and conva = GEN_REWRITE_CONV I [AND_CLAUSES] in
+  let rec conv tm =
+    (conv0 ORELSEC
+     (funpow 3 RAND_CONV num_CONV THENC
+      conv1 THENC
+      conv)) tm in
+  fun tm ->
+    match tm with
+       Comb(Comb(Const("bit",_),k),Comb(Const("word",_),n))
+       when is_numeral k && is_numeral n ->
+     (GEN_REWRITE_CONV I [BIT_WORD] THENC
+      BINOP2_CONV (RAND_CONV (!word_SIZE_CONV) THENC NUM_LT_CONV) conv THENC
+      conva) tm
+    | _ -> failwith "WORD_BIT_CONV";;
+
+let WORD_EQ_CONV =
+   let pth = prove
+   (`word(NUMERAL m):N word = (word(NUMERAL n):N word) <=>
+     val(word(NUMERAL m):N word) = val(word(NUMERAL n):N word)`,
+    REWRITE_TAC[VAL_EQ]) in
+  GEN_REWRITE_CONV I [pth] THENC BINOP_CONV WORD_VAL_CONV THENC NUM_EQ_CONV;;
+
+let WORD_ULT_CONV =
+  let pth = prove
+   (`word_ult (word(NUMERAL m):N word) (word(NUMERAL n):N word) <=>
+     val(word(NUMERAL m):N word) < val(word(NUMERAL n):N word)`,
+    REWRITE_TAC[word_ult; relational2]) in
+  GEN_REWRITE_CONV I [pth] THENC BINOP_CONV WORD_VAL_CONV THENC NUM_LT_CONV;;
+
+let WORD_ULE_CONV =
+  let pth = prove
+   (`word_ule (word(NUMERAL m):N word) (word(NUMERAL n):N word) <=>
+     val(word(NUMERAL m):N word) <= val(word(NUMERAL n):N word)`,
+    REWRITE_TAC[word_ule; relational2]) in
+  GEN_REWRITE_CONV I [pth] THENC BINOP_CONV WORD_VAL_CONV THENC NUM_LE_CONV;;
+
+let WORD_UGT_CONV =
+  let pth = prove
+   (`word_ugt (word(NUMERAL m):N word) (word(NUMERAL n):N word) <=>
+     val(word(NUMERAL m):N word) > val(word(NUMERAL n):N word)`,
+    REWRITE_TAC[word_ugt; relational2]) in
+  GEN_REWRITE_CONV I [pth] THENC BINOP_CONV WORD_VAL_CONV THENC NUM_GT_CONV;;
+
+let WORD_UGE_CONV =
+  let pth = prove
+   (`word_uge (word(NUMERAL m):N word) (word(NUMERAL n):N word) <=>
+     val(word(NUMERAL m):N word) >= val(word(NUMERAL n):N word)`,
+    REWRITE_TAC[word_uge; relational2]) in
+  GEN_REWRITE_CONV I [pth] THENC BINOP_CONV WORD_VAL_CONV THENC NUM_GE_CONV;;
+
+let WORD_ILT_CONV =
+  let pth = prove
+   (`word_ilt (word(NUMERAL m):N word) (word(NUMERAL n):N word) <=>
+     ival(word(NUMERAL m):N word) < ival(word(NUMERAL n):N word)`,
+    REWRITE_TAC[word_ilt; irelational2]) in
+  GEN_REWRITE_CONV I [pth] THENC BINOP_CONV WORD_IVAL_CONV THENC INT_LT_CONV;;
+
+let WORD_ILE_CONV =
+  let pth = prove
+   (`word_ile (word(NUMERAL m):N word) (word(NUMERAL n):N word) <=>
+     ival(word(NUMERAL m):N word) <= ival(word(NUMERAL n):N word)`,
+    REWRITE_TAC[word_ile; irelational2]) in
+  GEN_REWRITE_CONV I [pth] THENC BINOP_CONV WORD_IVAL_CONV THENC INT_LE_CONV;;
+
+let WORD_IGT_CONV =
+  let pth = prove
+   (`word_igt (word(NUMERAL m):N word) (word(NUMERAL n):N word) <=>
+     ival(word(NUMERAL m):N word) > ival(word(NUMERAL n):N word)`,
+    REWRITE_TAC[word_igt; irelational2]) in
+  GEN_REWRITE_CONV I [pth] THENC BINOP_CONV WORD_IVAL_CONV THENC INT_GT_CONV;;
+
+let WORD_IGE_CONV =
+  let pth = prove
+   (`word_ige (word(NUMERAL m):N word) (word(NUMERAL n):N word) <=>
+     ival(word(NUMERAL m):N word) >= ival(word(NUMERAL n):N word)`,
+    REWRITE_TAC[word_ige; irelational2]) in
+  GEN_REWRITE_CONV I [pth] THENC BINOP_CONV WORD_IVAL_CONV THENC INT_GE_CONV;;
+
+let WORD_ADD_CONV =
+  let pth = prove
+   (`word_add (word(NUMERAL m):N word) (word(NUMERAL n):N word) =
+     word((NUMERAL m + NUMERAL n) MOD (2 EXP dimindex(:N)))`,
+    REWRITE_TAC[word_add; modular; VAL_WORD; WORD_EQ; CONG] THEN
+    CONV_TAC MOD_DOWN_CONV THEN REWRITE_TAC[]) in
+  GEN_REWRITE_CONV I [pth] THENC
+  RAND_CONV
+   (BINOP2_CONV NUM_ADD_CONV (!word_POW2SIZE_CONV) THENC NUM_MOD_CONV);;
+
+let WORD_MUL_CONV =
+  let pth = prove
+   (`word_mul (word(NUMERAL m):N word) (word(NUMERAL n):N word) =
+     word((NUMERAL m * NUMERAL n) MOD (2 EXP dimindex(:N)))`,
+    REWRITE_TAC[word_mul; modular; VAL_WORD; WORD_EQ; CONG] THEN
+    CONV_TAC MOD_DOWN_CONV THEN REWRITE_TAC[]) in
+  GEN_REWRITE_CONV I [pth] THENC
+  RAND_CONV
+   (BINOP2_CONV NUM_MULT_CONV (!word_POW2SIZE_CONV) THENC NUM_MOD_CONV);;
+
+let WORD_SUB_CONV =
+  let pth = prove
+   (`word_sub (word(NUMERAL m):N word) (word(NUMERAL n):N word) =
+     (\p. word((NUMERAL m + (p - NUMERAL n MOD p)) MOD p))
+     (2 EXP dimindex(:N))`,
+    REWRITE_TAC[word_sub; modular; VAL_WORD; WORD_EQ; CONG] THEN
+    CONV_TAC MOD_DOWN_CONV THEN REWRITE_TAC[]) in
+  GEN_REWRITE_CONV I [pth] THENC
+  RAND_CONV(!word_POW2SIZE_CONV) THENC BETA_CONV THENC
+  RAND_CONV
+   (LAND_CONV
+    (RAND_CONV(RAND_CONV NUM_MOD_CONV THENC NUM_SUB_CONV) THENC
+     NUM_ADD_CONV) THENC
+    NUM_MOD_CONV);;
+
+let WORD_NEG_CONV =
+  let pth = prove
+   (`word_neg (word(NUMERAL n):N word) =
+     (\p. word((p - NUMERAL n MOD p) MOD p))
+     (2 EXP dimindex(:N))`,
+    REWRITE_TAC[word_neg; word_sub; modular; VAL_WORD; WORD_EQ; CONG] THEN
+    CONV_TAC MOD_DOWN_CONV THEN REWRITE_TAC[ADD_CLAUSES]) in
+  GEN_REWRITE_CONV I [pth] THENC
+  RAND_CONV(!word_POW2SIZE_CONV) THENC BETA_CONV THENC
+  RAND_CONV
+   (LAND_CONV
+    (RAND_CONV NUM_MOD_CONV THENC NUM_SUB_CONV) THENC
+    NUM_MOD_CONV);;
+
+let WORD_UDIV_CONV =
+  let pth = prove
+   (`word_udiv (word(NUMERAL m):N word) (word(NUMERAL n):N word) =
+     (\p. word((NUMERAL m MOD p) DIV (NUMERAL n MOD p)))
+     (2 EXP dimindex(:N))`,
+    REWRITE_TAC[GSYM VAL_EQ; VAL_WORD_UDIV; VAL_WORD] THEN
+    CONV_TAC SYM_CONV THEN MATCH_MP_TAC MOD_LT THEN MATCH_MP_TAC(ARITH_RULE
+     `m DIV n <= m /\ m < p ==> m DIV n < p`) THEN
+    SIMP_TAC[DIV_LE; DIVISION; EXP_EQ_0; ARITH_EQ]) in
+  GEN_REWRITE_CONV I [pth] THENC
+  RAND_CONV(!word_POW2SIZE_CONV) THENC BETA_CONV THENC
+  RAND_CONV(BINOP_CONV NUM_MOD_CONV THENC NUM_DIV_CONV);;
+
+let WORD_UMOD_CONV =
+  let pth = prove
+   (`word_umod (word(NUMERAL m):N word) (word(NUMERAL n):N word) =
+     (\p. word((NUMERAL m MOD p) MOD (NUMERAL n MOD p)))
+     (2 EXP dimindex(:N))`,
+    REWRITE_TAC[GSYM VAL_EQ; VAL_WORD_UMOD; VAL_WORD] THEN
+    CONV_TAC SYM_CONV THEN MATCH_MP_TAC MOD_LT THEN MATCH_MP_TAC(ARITH_RULE
+     `m MOD n <= m /\ m < p ==> m MOD n < p`) THEN
+    SIMP_TAC[MOD_LE; DIVISION; EXP_EQ_0; ARITH_EQ]) in
+  GEN_REWRITE_CONV I [pth] THENC
+  RAND_CONV(!word_POW2SIZE_CONV) THENC BETA_CONV THENC
+  RAND_CONV(BINOP_CONV NUM_MOD_CONV THENC NUM_MOD_CONV);;
+
+let WORD_UMAX_CONV =
+  let pth = prove
+   (`word_umax (word(NUMERAL m):N word) (word(NUMERAL n):N word) =
+     (\p. word(MAX (NUMERAL m MOD p) (NUMERAL n MOD p)))
+     (2 EXP dimindex(:N))`,
+    REWRITE_TAC[GSYM VAL_EQ; VAL_WORD_UMAX; VAL_WORD] THEN
+    CONV_TAC SYM_CONV THEN MATCH_MP_TAC MOD_LT THEN
+    REWRITE_TAC[ARITH_RULE `MAX a b < n <=> a < n /\ b < n`] THEN
+    SIMP_TAC[DIVISION; EXP_EQ_0; ARITH_EQ]) in
+  GEN_REWRITE_CONV I [pth] THENC
+  RAND_CONV(!word_POW2SIZE_CONV) THENC BETA_CONV THENC
+  RAND_CONV(BINOP_CONV NUM_MOD_CONV THENC NUM_MAX_CONV);;
+
+let WORD_UMIN_CONV =
+  let pth = prove
+   (`word_umin (word(NUMERAL m):N word) (word(NUMERAL n):N word) =
+     (\p. word(MIN (NUMERAL m MOD p) (NUMERAL n MOD p)))
+     (2 EXP dimindex(:N))`,
+    REWRITE_TAC[GSYM VAL_EQ; VAL_WORD_UMIN; VAL_WORD] THEN
+    CONV_TAC SYM_CONV THEN MATCH_MP_TAC MOD_LT THEN
+    REWRITE_TAC[ARITH_RULE `MIN a b < n <=> a < n \/ b < n`] THEN
+    SIMP_TAC[DIVISION; EXP_EQ_0; ARITH_EQ]) in
+  GEN_REWRITE_CONV I [pth] THENC
+  RAND_CONV(!word_POW2SIZE_CONV) THENC BETA_CONV THENC
+  RAND_CONV(BINOP_CONV NUM_MOD_CONV THENC NUM_MIN_CONV);;
+
+let WORD_IMAX_CONV =
+  let pth = prove
+   (`word_imax (word(NUMERAL m):N word) (word(NUMERAL n):N word) =
+     if ival(word(NUMERAL m):N word) <= ival(word(NUMERAL n):N word)
+     then word((NUMERAL n) MOD (2 EXP dimindex(:N)))
+     else word((NUMERAL m) MOD (2 EXP dimindex(:N)))`,
+    COND_CASES_TAC THEN
+    REWRITE_TAC[GSYM IVAL_EQ; IVAL_WORD_IMAX; WORD_MOD_SIZE] THEN
+    ASM_REWRITE_TAC[INT_MAX]) in
+  GEN_REWRITE_CONV I [pth] THENC
+  RATOR_CONV(LAND_CONV(BINOP_CONV WORD_IVAL_CONV THENC INT_LE_CONV)) THENC
+  GEN_REWRITE_CONV I [COND_CLAUSES] THENC
+  funpow 2 RAND_CONV (!word_POW2SIZE_CONV) THENC RAND_CONV NUM_MOD_CONV;;
+
+let WORD_IMIN_CONV =
+  let pth = prove
+   (`word_imin (word(NUMERAL m):N word) (word(NUMERAL n):N word) =
+     if ival(word(NUMERAL m):N word) <= ival(word(NUMERAL n):N word)
+     then word((NUMERAL m) MOD (2 EXP dimindex(:N)))
+     else word((NUMERAL n) MOD (2 EXP dimindex(:N)))`,
+    COND_CASES_TAC THEN
+    REWRITE_TAC[GSYM IVAL_EQ; IVAL_WORD_IMIN; WORD_MOD_SIZE] THEN
+    ASM_REWRITE_TAC[INT_MIN]) in
+  GEN_REWRITE_CONV I [pth] THENC
+  RATOR_CONV(LAND_CONV(BINOP_CONV WORD_IVAL_CONV THENC INT_LE_CONV)) THENC
+  GEN_REWRITE_CONV I [COND_CLAUSES] THENC
+  funpow 2 RAND_CONV (!word_POW2SIZE_CONV) THENC RAND_CONV NUM_MOD_CONV;;
+
+let WORD_SHL_CONV =
+  let pth = prove
+   (`word_shl (word(NUMERAL m):N word) (NUMERAL n) =
+     (\p. word((NUMERAL m * 2 EXP (NUMERAL n)) MOD p))
+     (2 EXP dimindex(:N))`,
+    REWRITE_TAC[word_shl; WORD_EQ; VAL_WORD; CONG] THEN
+    CONV_TAC MOD_DOWN_CONV THEN REFL_TAC) in
+  GEN_REWRITE_CONV I [pth] THENC
+  RAND_CONV (!word_POW2SIZE_CONV) THENC BETA_CONV THENC
+  RAND_CONV
+   (LAND_CONV
+     (RAND_CONV NUM_EXP_CONV THENC
+      NUM_MULT_CONV) THENC
+    NUM_MOD_CONV);;
+
+let WORD_USHR_CONV =
+  let pth = prove
+   (`word_ushr (word(NUMERAL m):N word) (NUMERAL n) =
+     (\p. word((NUMERAL m MOD p) DIV (2 EXP NUMERAL n) MOD p))
+     (2 EXP dimindex(:N))`,
+    REWRITE_TAC[word_ushr; WORD_EQ; VAL_WORD; CONG] THEN
+    CONV_TAC MOD_DOWN_CONV THEN REFL_TAC) in
+  GEN_REWRITE_CONV I [pth] THENC
+  RAND_CONV (!word_POW2SIZE_CONV) THENC BETA_CONV THENC
+  RAND_CONV
+   (LAND_CONV
+     (BINOP2_CONV NUM_MOD_CONV NUM_EXP_CONV THENC NUM_DIV_CONV) THENC
+    NUM_MOD_CONV);;
+
+let WORD_ISHR_CONV =
+  let pth = prove
+   (`word_ishr (word(NUMERAL m):N word) (NUMERAL n) =
+     iword (ival(word(NUMERAL m):N word) div &2 pow (NUMERAL n))`,
+    REWRITE_TAC[word_ishr]) in
+  GEN_REWRITE_CONV I [pth] THENC
+  RAND_CONV(BINOP2_CONV WORD_IVAL_CONV INT_POW_CONV THENC INT_DIV_CONV) THENC
+  WORD_IWORD_CONV;;
+
+let WORD_NOT_CONV =
+  let pth = prove
+   (`word_not(word n:N word) =
+     (\p. word(p - 1 - n MOD p)) (2 EXP dimindex(:N))`,
+    REWRITE_TAC[GSYM VAL_EQ; VAL_WORD_NOT; VAL_WORD] THEN
+    CONV_TAC SYM_CONV THEN MATCH_MP_TAC MOD_LT THEN
+    MATCH_MP_TAC(ARITH_RULE `~(p = 0) ==> p - 1 - n < p`) THEN
+    REWRITE_TAC[EXP_EQ_0; ARITH_EQ]) in
+  fun tm ->
+   (match tm with
+      Comb(Const("word_not",_),Comb(Const("word",_),n)) when is_numeral n ->
+     (GEN_REWRITE_CONV I [pth] THENC
+      RAND_CONV (!word_POW2SIZE_CONV) THENC BETA_CONV THENC
+      RAND_CONV(BINOP2_CONV NUM_SUB_CONV NUM_MOD_CONV THENC
+                NUM_SUB_CONV)) tm
+    | _ -> failwith "WORD_NOT_CONV");;
+
+let WORD_AND_CONV =
+  let pth = prove
+   (`?f. ((!n. f _0 n = _0) /\ (!m. f m _0 = _0)) /\
+         ((!m n. f (BIT0 m) (BIT0 n) = BIT0(f m n)) /\
+          (!m n. f (BIT0 m) (BIT1 n) = BIT0(f m n)) /\
+          (!m n. f (BIT1 m) (BIT0 n) = BIT0(f m n)) /\
+          (!m n. f (BIT1 m) (BIT1 n) = BIT1(f m n))) /\
+         (!m n. word_and (word(NUMERAL m):N word) (word(NUMERAL n)) =
+                word(NUMERAL(f m n)))`,
+    MP_TAC(prove_general_recursive_function_exists
+     `?f. !m n. f m n =
+                if m = 0 then 0 else if n = 0 then 0
+                else (if m MOD 2 = 1 /\ n MOD 2 = 1 then 1 else 0) +
+                     2 * f (m DIV 2) (n DIV 2)`) THEN
+    MATCH_MP_TAC MONO_EXISTS THEN X_GEN_TAC `f:num->num->num` THEN
+    DISCH_TAC THEN
+    SUBGOAL_THEN
+     `(!n. f 0 n = 0) /\ (!m. f m 0 = 0) /\
+      (!m n. f (2 * m) (2 * n) = 2 * f m n) /\
+      (!m n. f (2 * m + 1) (2 * n) = 2 * f m n) /\
+      (!m n. f (2 * m) (2 * n + 1) = 2 * f m n) /\
+      (!m n. f (2 * m + 1) (2 * n + 1) = 2 * f m n + 1)`
+    MP_TAC THENL
+     [REPEAT STRIP_TAC THEN
+      FIRST_ASSUM(fun th -> GEN_REWRITE_TAC LAND_CONV [th]) THEN
+      REWRITE_TAC[ARITH_RULE `(2 * n) DIV 2 = n /\ (2 * n + 1) DIV 2 = n`;
+                  ONCE_REWRITE_RULE[MULT_SYM] MOD_MULT_ADD;
+                 MOD_MULT; ADD_EQ_0; MULT_EQ_0] THEN
+      CONV_TAC NUM_REDUCE_CONV THEN
+      REWRITE_TAC[ADD_CLAUSES; ARITH_RULE `1 + 2 * n = 2 * n + 1`] THEN
+      REPEAT(COND_CASES_TAC THEN REWRITE_TAC[]) THEN
+      REWRITE_TAC[ARITH_RULE `0 = 2 * n <=> n = 0`] THEN
+      FIRST_X_ASSUM(fun th -> GEN_REWRITE_TAC LAND_CONV [th]) THEN
+      ASM_REWRITE_TAC[COND_ID];
+      FIRST_X_ASSUM(K ALL_TAC) THEN STRIP_TAC] THEN
+    CONJ_TAC THENL [ASM_MESON_TAC[NUMERAL]; ALL_TAC] THEN CONJ_TAC THENL
+     [REWRITE_TAC[BIT0; BIT1] THEN ASM_REWRITE_TAC[GSYM MULT_2; ADD1];
+      REWRITE_TAC[NUMERAL]] THEN
+    REWRITE_TAC[WORD_EQ_BITS; BIT_WORD_AND; BIT_WORD] THEN
+    SIMP_TAC[TAUT `(p /\ q <=> p /\ r) <=> (p ==> (q <=> r))`] THEN
+    MATCH_MP_TAC BINARY_INDUCT THEN ASM_REWRITE_TAC[DIV_0; ODD] THEN
+    X_GEN_TAC `m:num` THEN DISCH_TAC THEN CONJ_TAC THEN
+    MATCH_MP_TAC BINARY_INDUCT THEN ASM_REWRITE_TAC[DIV_0; ODD] THEN
+    X_GEN_TAC `n:num` THEN DISCH_THEN(K ALL_TAC) THEN CONJ_TAC THEN
+    INDUCT_TAC THEN REWRITE_TAC[EXP; DIV_1; ODD_MULT; ARITH; ODD_ADD] THEN
+    DISCH_TAC THEN REWRITE_TAC[GSYM DIV_DIV] THEN
+    REWRITE_TAC[ARITH_RULE `(2 * n) DIV 2 = n /\ (2 * n + 1) DIV 2 = n`;
+                MOD_MULT; ONCE_REWRITE_RULE[MULT_SYM] MOD_MULT_ADD] THEN
+    FIRST_X_ASSUM MATCH_MP_TAC THEN ASM_ARITH_TAC)
+  and qth = prove
+   (`BIT0 _0 = _0`,
+    REWRITE_TAC[ARITH_ZERO])
+  and nty = `:N` in
+  fun tm ->
+    (match tm with
+      Comb(Comb(Const("word_and",_),
+                Comb(Const("word",_),m)),
+           Comb(Const("word",_),n))
+          when is_numeral m && is_numeral n ->
+       let th1 = INST_TYPE
+          [hd(snd(dest_type(type_of(rand tm)))),nty] pth in
+       let f,bod = dest_exists(concl th1) in
+       let pth_base,th2 = CONJ_PAIR(ASSUME bod) in
+       let pth_step,pth_trans = CONJ_PAIR th2 in
+       let base_conv = GEN_REWRITE_CONV I [pth_base]
+       and step_conv = GEN_REWRITE_CONV I [pth_step]
+       and fix_conv = GEN_REWRITE_CONV TRY_CONV [qth] in
+       let rec conv t =
+         (base_conv ORELSEC
+          (step_conv THENC RAND_CONV conv THENC fix_conv)) t in
+       let th3 = REWR_CONV pth_trans tm in
+       let th4 = CONV_RULE(funpow 3 RAND_CONV conv) th3 in
+       let th5 = PROVE_HYP th1 (SIMPLE_CHOOSE f th4) in
+       CONV_RULE(RAND_CONV WORD_WORD_CONV) th5
+     | _ -> failwith "WORD_AND_CONV");;
+
+let WORD_OR_CONV =
+  let pth = prove
+   (`?f. ((!n. f _0 n = n) /\ (!m. f m _0 = m)) /\
+         ((!m n. f (BIT0 m) (BIT0 n) = BIT0(f m n)) /\
+          (!m n. f (BIT0 m) (BIT1 n) = BIT1(f m n)) /\
+          (!m n. f (BIT1 m) (BIT0 n) = BIT1(f m n)) /\
+          (!m n. f (BIT1 m) (BIT1 n) = BIT1(f m n))) /\
+         (!m n. word_or (word(NUMERAL m):N word) (word(NUMERAL n)) =
+                word(NUMERAL(f m n)))`,
+    MP_TAC(prove_general_recursive_function_exists
+     `?f. !m n. f m n =
+                if m = 0 then n else if n = 0 then m
+                else (if m MOD 2 = 1 \/ n MOD 2 = 1 then 1 else 0) +
+                     2 * f (m DIV 2) (n DIV 2)`) THEN
+    MATCH_MP_TAC MONO_EXISTS THEN X_GEN_TAC `f:num->num->num` THEN
+    DISCH_TAC THEN
+    SUBGOAL_THEN
+     `(!n. f 0 n = n) /\ (!m. f m 0 = m) /\
+      (!m n. f (2 * m) (2 * n) = 2 * f m n) /\
+      (!m n. f (2 * m + 1) (2 * n) = 2 * f m n + 1) /\
+      (!m n. f (2 * m) (2 * n + 1) = 2 * f m n + 1) /\
+      (!m n. f (2 * m + 1) (2 * n + 1) = 2 * f m n + 1)`
+    MP_TAC THENL
+     [REPEAT STRIP_TAC THEN
+      FIRST_ASSUM(fun th -> GEN_REWRITE_TAC LAND_CONV [th]) THEN
+      REWRITE_TAC[ARITH_RULE `(2 * n) DIV 2 = n /\ (2 * n + 1) DIV 2 = n`;
+                  ONCE_REWRITE_RULE[MULT_SYM] MOD_MULT_ADD;
+                 MOD_MULT; ADD_EQ_0; MULT_EQ_0] THEN
+      CONV_TAC NUM_REDUCE_CONV THEN
+      REWRITE_TAC[ADD_CLAUSES; ARITH_RULE `1 + 2 * n = 2 * n + 1`] THEN
+      REPEAT(COND_CASES_TAC THEN REWRITE_TAC[]) THEN
+      ONCE_REWRITE_TAC[EQ_SYM_EQ] THEN TRY(FIRST_ASSUM ACCEPT_TAC) THEN
+      TRY(AP_THM_TAC THEN AP_TERM_TAC) THEN AP_TERM_TAC THEN
+      FIRST_X_ASSUM(fun th -> GEN_REWRITE_TAC LAND_CONV [th]) THEN
+      ASM_REWRITE_TAC[COND_ID] THEN MESON_TAC[];
+      FIRST_X_ASSUM(K ALL_TAC) THEN STRIP_TAC] THEN
+    CONJ_TAC THENL [ASM_MESON_TAC[NUMERAL]; ALL_TAC] THEN CONJ_TAC THENL
+     [REWRITE_TAC[BIT0; BIT1] THEN ASM_REWRITE_TAC[GSYM MULT_2; ADD1];
+      REWRITE_TAC[NUMERAL]] THEN
+    REWRITE_TAC[WORD_EQ_BITS; BIT_WORD_OR; BIT_WORD] THEN
+    SIMP_TAC[TAUT `(p /\ q <=> p /\ r) <=> (p ==> (q <=> r))`] THEN
+    MATCH_MP_TAC BINARY_INDUCT THEN ASM_REWRITE_TAC[DIV_0; ODD] THEN
+    X_GEN_TAC `m:num` THEN DISCH_TAC THEN CONJ_TAC THEN
+    MATCH_MP_TAC BINARY_INDUCT THEN ASM_REWRITE_TAC[DIV_0; ODD] THEN
+    X_GEN_TAC `n:num` THEN DISCH_THEN(K ALL_TAC) THEN CONJ_TAC THEN
+    INDUCT_TAC THEN REWRITE_TAC[EXP; DIV_1; ODD_MULT; ARITH; ODD_ADD] THEN
+    DISCH_TAC THEN REWRITE_TAC[GSYM DIV_DIV] THEN
+    REWRITE_TAC[ARITH_RULE `(2 * n) DIV 2 = n /\ (2 * n + 1) DIV 2 = n`;
+                MOD_MULT; ONCE_REWRITE_RULE[MULT_SYM] MOD_MULT_ADD] THEN
+    FIRST_X_ASSUM MATCH_MP_TAC THEN ASM_ARITH_TAC)
+  and qth = prove
+   (`BIT0 _0 = _0`,
+    REWRITE_TAC[ARITH_ZERO])
+  and nty = `:N` in
+  fun tm ->
+    (match tm with
+      Comb(Comb(Const("word_or",_),
+                Comb(Const("word",_),m)),
+           Comb(Const("word",_),n))
+          when is_numeral m && is_numeral n ->
+       let th1 = INST_TYPE
+          [hd(snd(dest_type(type_of(rand tm)))),nty] pth in
+       let f,bod = dest_exists(concl th1) in
+       let pth_base,th2 = CONJ_PAIR(ASSUME bod) in
+       let pth_step,pth_trans = CONJ_PAIR th2 in
+       let base_conv = GEN_REWRITE_CONV I [pth_base]
+       and step_conv = GEN_REWRITE_CONV I [pth_step]
+       and fix_conv = GEN_REWRITE_CONV TRY_CONV [qth] in
+       let rec conv t =
+         (base_conv ORELSEC
+          (step_conv THENC RAND_CONV conv THENC fix_conv)) t in
+       let th3 = REWR_CONV pth_trans tm in
+       let th4 = CONV_RULE(funpow 3 RAND_CONV conv) th3 in
+       let th5 = PROVE_HYP th1 (SIMPLE_CHOOSE f th4) in
+       CONV_RULE(RAND_CONV WORD_WORD_CONV) th5
+     | _ -> failwith "WORD_OR_CONV");;
+
+let WORD_XOR_CONV =
+  let pth = prove
+   (`?f. ((!n. f _0 n = n) /\ (!m. f m _0 = m)) /\
+         ((!m n. f (BIT0 m) (BIT0 n) = BIT0(f m n)) /\
+          (!m n. f (BIT0 m) (BIT1 n) = BIT1(f m n)) /\
+          (!m n. f (BIT1 m) (BIT0 n) = BIT1(f m n)) /\
+          (!m n. f (BIT1 m) (BIT1 n) = BIT0(f m n))) /\
+         (!m n. word_xor (word(NUMERAL m):N word) (word(NUMERAL n)) =
+                word(NUMERAL(f m n)))`,
+    MP_TAC(prove_general_recursive_function_exists
+     `?f. !m n. f m n =
+                if m = 0 then n else if n = 0 then m
+                else (if m MOD 2 = 1 <=> n MOD 2 = 1 then 0 else 1) +
+                     2 * f (m DIV 2) (n DIV 2)`) THEN
+    MATCH_MP_TAC MONO_EXISTS THEN X_GEN_TAC `f:num->num->num` THEN
+    DISCH_TAC THEN
+    SUBGOAL_THEN
+     `(!n. f 0 n = n) /\ (!m. f m 0 = m) /\
+      (!m n. f (2 * m) (2 * n) = 2 * f m n) /\
+      (!m n. f (2 * m + 1) (2 * n) = 2 * f m n + 1) /\
+      (!m n. f (2 * m) (2 * n + 1) = 2 * f m n + 1) /\
+      (!m n. f (2 * m + 1) (2 * n + 1) = 2 * f m n)`
+    MP_TAC THENL
+     [REPEAT STRIP_TAC THEN
+      FIRST_ASSUM(fun th -> GEN_REWRITE_TAC LAND_CONV [th]) THEN
+      REWRITE_TAC[ARITH_RULE `(2 * n) DIV 2 = n /\ (2 * n + 1) DIV 2 = n`;
+                  ONCE_REWRITE_RULE[MULT_SYM] MOD_MULT_ADD;
+                 MOD_MULT; ADD_EQ_0; MULT_EQ_0] THEN
+      CONV_TAC NUM_REDUCE_CONV THEN
+      REWRITE_TAC[ADD_CLAUSES; ARITH_RULE `1 + 2 * n = 2 * n + 1`] THEN
+      REPEAT(COND_CASES_TAC THEN REWRITE_TAC[]) THEN
+      ONCE_REWRITE_TAC[EQ_SYM_EQ] THEN TRY(FIRST_ASSUM ACCEPT_TAC) THEN
+      TRY(AP_THM_TAC THEN AP_TERM_TAC) THEN AP_TERM_TAC THEN
+      FIRST_X_ASSUM(fun th -> GEN_REWRITE_TAC LAND_CONV [th]) THEN
+      ASM_REWRITE_TAC[COND_ID] THEN MESON_TAC[];
+      FIRST_X_ASSUM(K ALL_TAC) THEN STRIP_TAC] THEN
+    CONJ_TAC THENL [ASM_MESON_TAC[NUMERAL]; ALL_TAC] THEN CONJ_TAC THENL
+     [REWRITE_TAC[BIT0; BIT1] THEN ASM_REWRITE_TAC[GSYM MULT_2; ADD1];
+      REWRITE_TAC[NUMERAL]] THEN
+    REWRITE_TAC[WORD_EQ_BITS; BIT_WORD_XOR; BIT_WORD] THEN
+    SIMP_TAC[TAUT `(p /\ q <=> p /\ r) <=> (p ==> (q <=> r))`] THEN
+    MATCH_MP_TAC BINARY_INDUCT THEN ASM_REWRITE_TAC[DIV_0; ODD] THEN
+    X_GEN_TAC `m:num` THEN DISCH_TAC THEN CONJ_TAC THEN
+    MATCH_MP_TAC BINARY_INDUCT THEN ASM_REWRITE_TAC[DIV_0; ODD] THEN
+    X_GEN_TAC `n:num` THEN DISCH_THEN(K ALL_TAC) THEN CONJ_TAC THEN
+    INDUCT_TAC THEN REWRITE_TAC[EXP; DIV_1; ODD_MULT; ARITH; ODD_ADD] THEN
+    DISCH_TAC THEN REWRITE_TAC[GSYM DIV_DIV] THEN
+    REWRITE_TAC[ARITH_RULE `(2 * n) DIV 2 = n /\ (2 * n + 1) DIV 2 = n`;
+                MOD_MULT; ONCE_REWRITE_RULE[MULT_SYM] MOD_MULT_ADD] THEN
+    FIRST_X_ASSUM MATCH_MP_TAC THEN ASM_ARITH_TAC)
+  and qth = prove
+   (`BIT0 _0 = _0`,
+    REWRITE_TAC[ARITH_ZERO])
+  and nty = `:N` in
+  fun tm ->
+    (match tm with
+      Comb(Comb(Const("word_xor",_),
+                Comb(Const("word",_),m)),
+           Comb(Const("word",_),n))
+          when is_numeral m && is_numeral n ->
+       let th1 = INST_TYPE
+          [hd(snd(dest_type(type_of(rand tm)))),nty] pth in
+       let f,bod = dest_exists(concl th1) in
+       let pth_base,th2 = CONJ_PAIR(ASSUME bod) in
+       let pth_step,pth_trans = CONJ_PAIR th2 in
+       let base_conv = GEN_REWRITE_CONV I [pth_base]
+       and step_conv = GEN_REWRITE_CONV I [pth_step]
+       and fix_conv = GEN_REWRITE_CONV TRY_CONV [qth] in
+       let rec conv t =
+         (base_conv ORELSEC
+          (step_conv THENC RAND_CONV conv THENC fix_conv)) t in
+       let th3 = REWR_CONV pth_trans tm in
+       let th4 = CONV_RULE(funpow 3 RAND_CONV conv) th3 in
+       let th5 = PROVE_HYP th1 (SIMPLE_CHOOSE f th4) in
+       CONV_RULE(RAND_CONV WORD_WORD_CONV) th5
+     | _ -> failwith "WORD_XOR_CONV");;
+
+let WORD_ROL_CONV =
+  let pth = prove
+   (`word_rol (word(NUMERAL m):N word) n =
+     (\n. word_or (word_shl (word(NUMERAL m):N word) n)
+                  (word_ushr (word(NUMERAL m):N word) (dimindex (:N) - n)))
+     (n MOD dimindex(:N))`,
+    REWRITE_TAC[] THEN
+    GEN_REWRITE_TAC LAND_CONV [WORD_ROL_MOD] THEN
+    SIMP_TAC[WORD_ROL_SHIFTS; DIMINDEX_NONZERO; DIVISION; LT_IMP_LE]) in
+  GEN_REWRITE_CONV I [pth] THENC
+  (RAND_CONV o RAND_CONV) (!word_SIZE_CONV) THENC
+  RAND_CONV NUM_MOD_CONV THENC NUM_REDUCE_CONV THENC
+  BINOP2_CONV WORD_SHL_CONV
+              ((RAND_CONV o LAND_CONV) (!word_SIZE_CONV) THENC
+               RAND_CONV NUM_SUB_CONV THENC WORD_USHR_CONV) THENC
+  WORD_OR_CONV;;
+
+let WORD_ROR_CONV =
+  let pth = prove
+   (`word_ror (word(NUMERAL m):N word) n =
+     (\n. word_or (word_ushr (word(NUMERAL m):N word) n)
+                  (word_shl (word(NUMERAL m):N word) (dimindex (:N) - n)))
+     (n MOD dimindex(:N))`,
+    REWRITE_TAC[] THEN
+    GEN_REWRITE_TAC LAND_CONV [WORD_ROR_MOD] THEN
+    SIMP_TAC[WORD_ROR_SHIFTS; DIMINDEX_NONZERO; DIVISION; LT_IMP_LE]) in
+  GEN_REWRITE_CONV I [pth] THENC
+  (RAND_CONV o RAND_CONV) (!word_SIZE_CONV) THENC
+  RAND_CONV NUM_MOD_CONV THENC NUM_REDUCE_CONV THENC
+  BINOP2_CONV WORD_USHR_CONV
+              ((RAND_CONV o LAND_CONV) (!word_SIZE_CONV) THENC
+               RAND_CONV NUM_SUB_CONV THENC WORD_SHL_CONV) THENC
+  WORD_OR_CONV;;
+
+let WORD_ZX_CONV =
+  let pth = prove
+   (`(word_zx:M word->N word) (word (NUMERAL n)) =
+     word (NUMERAL n MOD (2 EXP (MIN (dimindex(:M)) (dimindex(:N)))))`,
+    REWRITE_TAC[GSYM VAL_EQ; VAL_WORD_ZX_GEN; VAL_WORD] THEN
+    MESON_TAC[MOD_MOD_EXP_MIN; MOD_MOD_REFL]) in
+  GEN_REWRITE_CONV I [pth] THENC
+  RAND_CONV
+   (RAND_CONV
+     (RAND_CONV(BINOP_CONV (!word_SIZE_CONV) THENC
+                NUM_MIN_CONV) THENC
+      NUM_EXP_CONV) THENC
+    NUM_MOD_CONV);;
+
+let WORD_SX_CONV =
+  let pth = prove
+   (`(word_sx:M word->N word) (word (NUMERAL n)) =
+     iword(ival(word(NUMERAL n):M word))`,
+    REWRITE_TAC[word_sx]) in
+  GEN_REWRITE_CONV I [pth] THENC
+  RAND_CONV WORD_IVAL_CONV THENC
+  WORD_IWORD_CONV;;
+
+let WORD_CAND_CONV =
+ let pth = prove
+  (`word_cand (word(NUMERAL m):N word) (word(NUMERAL n):N word) =
+    if word(NUMERAL m):N word = word 0 \/
+       word(NUMERAL n):N word = word 0
+    then word 0 else word 1`,
+   REWRITE_TAC[WORD_CAND]) in
+  GEN_REWRITE_CONV I [pth] THENC
+  RATOR_CONV(LAND_CONV
+   (BINOP_CONV WORD_EQ_CONV THENC
+    GEN_REWRITE_CONV I [OR_CLAUSES])) THENC
+  GEN_REWRITE_CONV I [COND_CLAUSES];;
+
+let WORD_COR_CONV =
+ let pth = prove
+  (`word_cor (word(NUMERAL m):N word) (word(NUMERAL n):N word) =
+    if word(NUMERAL m):N word = word 0 /\
+       word(NUMERAL n):N word = word 0
+    then word 0 else word 1`,
+   REWRITE_TAC[WORD_COR]) in
+  GEN_REWRITE_CONV I [pth] THENC
+  RATOR_CONV(LAND_CONV
+   (BINOP_CONV WORD_EQ_CONV THENC
+    GEN_REWRITE_CONV I [AND_CLAUSES])) THENC
+  GEN_REWRITE_CONV I [COND_CLAUSES];;
+
+let WORD_JOIN_CONV =
+ let pth = prove
+   (`(word_join:(M)word->(N)word->(P)word)
+     (word(NUMERAL m)) (word(NUMERAL n)) =
+     word((2 EXP dimindex(:N) * NUMERAL m MOD 2 EXP dimindex(:M) +
+           NUMERAL n MOD 2 EXP dimindex(:N)) MOD
+          2 EXP dimindex(:P))`,
+    REWRITE_TAC[GSYM VAL_EQ; VAL_WORD_JOIN; VAL_WORD; MOD_MOD_REFL]) in
+  GEN_REWRITE_CONV I [pth] THENC
+  RAND_CONV
+   (BINOP2_CONV
+      (BINOP2_CONV
+         (BINOP2_CONV
+           (!word_POW2SIZE_CONV)
+           (RAND_CONV(!word_POW2SIZE_CONV) THENC NUM_MOD_CONV) THENC
+          NUM_MULT_CONV)
+         (RAND_CONV(!word_POW2SIZE_CONV) THENC NUM_MOD_CONV)  THENC
+       NUM_ADD_CONV)
+      (!word_POW2SIZE_CONV) THENC
+    NUM_MOD_CONV);;
+
+let WORD_SUBWORD_CONV =
+  let pth = prove
+   (`word_subword (word(NUMERAL m):M word) (NUMERAL p,NUMERAL q):N word =
+     word((val(word(NUMERAL m):M word) DIV 2 EXP NUMERAL p) MOD
+           2 EXP MIN (NUMERAL q) (dimindex (:N)))`,
+    REWRITE_TAC[word_subword; GSYM MOD_MOD_EXP_MIN] THEN
+    REWRITE_TAC[WORD_EQ; CONG; MOD_MOD_REFL]) in
+  GEN_REWRITE_CONV I [pth] THENC
+  RAND_CONV
+   (BINOP2_CONV
+     (BINOP2_CONV WORD_VAL_CONV NUM_EXP_CONV THENC NUM_DIV_CONV)
+     (RAND_CONV (RAND_CONV (!word_SIZE_CONV) THENC NUM_MIN_CONV) THENC
+      NUM_EXP_CONV) THENC
+    NUM_MOD_CONV);;
+
+let WORD_BITS_OF_WORD_CONV =
+  let pth = prove
+   (`?f. (!i. f i _0 = {} /\
+              (!n. f i (BIT0 n) = f (i + 1) n) /\
+              (!n. f i (BIT1 n) = i INSERT f (i + 1) n)) /\
+         (!w:N word. bits_of_word w = f 0 (val w))`,
+    MP_TAC(prove_general_recursive_function_exists
+     `?f. !i n. f i n =
+                  if n = 0 then {}
+             else if n MOD 2 = 1 then i INSERT f (i + 1) (n DIV 2)
+             else f (i + 1) (n DIV 2)`) THEN
+    MATCH_MP_TAC MONO_EXISTS THEN X_GEN_TAC `f:num->num->num->bool` THEN
+    DISCH_TAC THEN
+    GEN_REWRITE_TAC
+     (LAND_CONV o BINDER_CONV o LAND_CONV o LAND_CONV o RAND_CONV)
+     [GSYM NUMERAL] THEN
+    GEN_REWRITE_TAC (LAND_CONV o BINDER_CONV o RAND_CONV o BINOP_CONV o
+                     BINDER_CONV o LAND_CONV o RAND_CONV)
+     [BIT0; BIT1] THEN
+    REWRITE_TAC[ADD1; GSYM MULT_2] THEN MATCH_MP_TAC(TAUT
+     `p /\ (p ==> q) ==> p /\ q`) THEN
+    CONJ_TAC THENL
+     [REPEAT STRIP_TAC THEN FIRST_ASSUM(fun th ->
+        GEN_REWRITE_TAC LAND_CONV [th]) THEN
+      REWRITE_TAC[ADD_EQ_0; MULT_EQ_0; ARITH_EQ; ARITH_RULE
+       `(2 * n + 1) DIV 2 = n /\ (2 * n) DIV 2 = n`] THEN
+      REWRITE_TAC[MOD_MULT] THEN
+      ONCE_REWRITE_TAC[MULT_SYM] THEN REWRITE_TAC[MOD_MULT_ADD] THEN
+      CONV_TAC NUM_REDUCE_CONV THEN ASM_MESON_TAC[];
+      POP_ASSUM(K ALL_TAC) THEN
+      REWRITE_TAC[FORALL_AND_THM] THEN STRIP_TAC] THEN
+    X_GEN_TAC `w:N word` THEN REWRITE_TAC[EXTENSION] THEN
+    SUBGOAL_THEN
+     `!k i. i IN f k (val w) <=> k <= i /\ (i - k) IN bits_of_word(w:N word)`
+    MP_TAC THENL [ALL_TAC; MESON_TAC[SUB_0; LE_0]] THEN
+    REWRITE_TAC[bits_of_word; BIT_VAL] THEN
+    SPEC_TAC(`val(w:N word)`,`n:num`) THEN
+    MATCH_MP_TAC BINARY_INDUCT THEN ASM_REWRITE_TAC[IN_ELIM_THM] THEN
+    REWRITE_TAC[DIV_0; NOT_IN_EMPTY; ARITH] THEN
+    X_GEN_TAC `n:num` THEN DISCH_TAC THEN
+    ASM_REWRITE_TAC[IN_INSERT; AND_FORALL_THM] THEN
+    MAP_EVERY X_GEN_TAC [`k:num`; `i:num`] THEN
+    ASM_CASES_TAC `i:num = k` THEN
+    ASM_REWRITE_TAC[LE_REFL; SUB_REFL; ARITH_RULE `~(k + 1 <= k)`] THEN
+    REWRITE_TAC[EXP; DIV_1; ODD_ADD; ODD_MULT; ARITH] THEN
+    ASM_CASES_TAC `k:num <= i` THEN ASM_REWRITE_TAC[] THENL
+     [ALL_TAC; ASM_ARITH_TAC] THEN
+    ASM_CASES_TAC `k + 1 <= i` THEN ASM_REWRITE_TAC[] THENL
+     [ALL_TAC; ASM_ARITH_TAC] THEN
+    SUBGOAL_THEN `i - k = SUC(i - (k + 1))` SUBST1_TAC THENL
+     [ASM_ARITH_TAC; REWRITE_TAC[EXP; GSYM DIV_DIV]] THEN
+    REWRITE_TAC[ARITH_RULE `(2 * n + 1) DIV 2 = n /\ (2 * n) DIV 2 = n`])
+  and nty = `:N` in
+  fun tm ->
+    (match tm with
+      Comb(Const("bits_of_word",_),Comb(Const("word",_),n))
+          when is_numeral n ->
+       let th1 = INST_TYPE
+          [hd(snd(dest_type(type_of(rand tm)))),nty] pth in
+       let f,bod = dest_exists(concl th1) in
+       let pth_clauses,th2 = CONJ_PAIR(ASSUME bod) in
+       let pth_z,pth_o = CONJ_PAIR(SPEC_ALL pth_clauses) in
+       let pth_0,pth_1 = CONJ_PAIR pth_o in
+       let conv_z = GEN_REWRITE_CONV I [pth_z]
+       and conv_0 = GEN_REWRITE_CONV I [pth_0]
+       and conv_1 = GEN_REWRITE_CONV I [pth_1] in
+       let rec conv t =
+        (conv_z ORELSEC
+         (conv_0 THENC LAND_CONV NUM_ADD_CONV THENC conv) ORELSEC
+         (conv_1 THENC RAND_CONV(LAND_CONV NUM_ADD_CONV THENC conv))) t in
+       let th3 = REWR_CONV th2 tm in
+       let th4 = CONV_RULE(RAND_CONV(RAND_CONV WORD_VAL_CONV)) th3 in
+       let th5 = GEN_REWRITE_RULE (RAND_CONV o RAND_CONV) [NUMERAL] th4 in
+       let th6 = CONV_RULE(RAND_CONV conv) th5 in
+       PROVE_HYP th1 (SIMPLE_CHOOSE f th6)
+     | _ -> failwith "WORD_BITS_OF_WORD_CONV");;
+
+let WORD_POPCOUNT_CONV =
+  let pth = prove
+   (`?f. (f _0 = 0 /\
+          (!n. f (BIT0 n) = f n) /\
+          (!n. f (BIT1 n) = SUC(f n))) /\
+         (!w:N word. word_popcount w = f (val w))`,
+    MP_TAC(prove_general_recursive_function_exists
+     `?f. !n. f n =
+                  if n = 0 then 0
+             else if n MOD 2 = 1 then SUC(f (n DIV 2))
+             else f (n DIV 2)`) THEN
+    MATCH_MP_TAC MONO_EXISTS THEN X_GEN_TAC `f:num->num` THEN
+    DISCH_TAC THEN
+    GEN_REWRITE_TAC
+     (LAND_CONV o LAND_CONV o LAND_CONV o RAND_CONV)
+     [GSYM NUMERAL] THEN
+    GEN_REWRITE_TAC (LAND_CONV o RAND_CONV o BINOP_CONV o
+                     BINDER_CONV o LAND_CONV o RAND_CONV)
+     [BIT0; BIT1] THEN
+    REWRITE_TAC[ADD1; GSYM MULT_2] THEN MATCH_MP_TAC(TAUT
+     `p /\ (p ==> q) ==> p /\ q`) THEN
+    CONJ_TAC THENL
+     [REPEAT STRIP_TAC THEN FIRST_ASSUM(fun th ->
+        GEN_REWRITE_TAC LAND_CONV [th]) THEN
+      REWRITE_TAC[ADD_EQ_0; MULT_EQ_0; ARITH_EQ; ARITH_RULE
+       `(2 * n + 1) DIV 2 = n /\ (2 * n) DIV 2 = n`] THEN
+      REWRITE_TAC[MOD_MULT] THEN
+      ONCE_REWRITE_TAC[MULT_SYM] THEN REWRITE_TAC[MOD_MULT_ADD] THEN
+      CONV_TAC NUM_REDUCE_CONV THEN ASM_MESON_TAC[ADD1];
+      POP_ASSUM(K ALL_TAC) THEN
+      REWRITE_TAC[FORALL_AND_THM] THEN STRIP_TAC] THEN
+    X_GEN_TAC `w:N word` THEN REWRITE_TAC[word_popcount] THEN
+    REWRITE_TAC[bits_of_word; BIT_VAL] THEN
+    SUBGOAL_THEN `!n. {i | ODD(n DIV 2 EXP i)} HAS_SIZE f n` MP_TAC THENL
+     [ALL_TAC; SIMP_TAC[HAS_SIZE]] THEN
+    MATCH_MP_TAC BINARY_INDUCT THEN
+    ASM_REWRITE_TAC[HAS_SIZE; DIV_0; ODD; EMPTY_GSPEC;
+                    FINITE_EMPTY; CARD_CLAUSES] THEN
+    X_GEN_TAC `n:num` THEN STRIP_TAC THEN
+    SUBGOAL_THEN
+     `!P. {i | P i} = {i | i = 0 /\ P 0} UNION IMAGE SUC {i | P(SUC i)}`
+     (fun th -> ONCE_REWRITE_TAC[th])
+    THENL
+     [REWRITE_TAC[EXTENSION; IN_UNION; IN_ELIM_THM; IN_IMAGE] THEN
+      MESON_TAC[num_CASES];
+      REWRITE_TAC[EXP; DIV_1; ODD_ADD; ODD_MULT; ARITH]] THEN
+    REWRITE_TAC[EMPTY_GSPEC; SING_GSPEC; GSYM DIV_DIV] THEN
+    REWRITE_TAC[ARITH_RULE `(2 * n + 1) DIV 2 = n /\ (2 * n) DIV 2 = n`] THEN
+    REWRITE_TAC[UNION_EMPTY; INSERT_UNION_EQ] THEN
+    ASM_SIMP_TAC[FINITE_INSERT; FINITE_IMAGE; CARD_CLAUSES] THEN
+    REWRITE_TAC[IN_IMAGE; NOT_SUC; ADD1; EQ_ADD_RCANCEL] THEN
+    ASM_SIMP_TAC[CARD_IMAGE_INJ; SUC_INJ])
+  and nty = `:N` in
+  fun tm ->
+    (match tm with
+      Comb(Const("word_popcount",_),Comb(Const("word",_),n))
+          when is_numeral n ->
+       let th1 = INST_TYPE
+          [hd(snd(dest_type(type_of(rand tm)))),nty] pth in
+       let f,bod = dest_exists(concl th1) in
+       let pth_clauses,th2 = CONJ_PAIR(ASSUME bod) in
+       let pth_z,pth_o = CONJ_PAIR(SPEC_ALL pth_clauses) in
+       let pth_0,pth_1 = CONJ_PAIR pth_o in
+       let conv_z = GEN_REWRITE_CONV I [pth_z]
+       and conv_0 = GEN_REWRITE_CONV I [pth_0]
+       and conv_1 = GEN_REWRITE_CONV I [pth_1] in
+       let rec conv t =
+        (conv_z ORELSEC
+         (conv_0 THENC conv) ORELSEC
+         (conv_1 THENC RAND_CONV conv THENC NUM_SUC_CONV)) t in
+       let th3 = REWR_CONV th2 tm in
+       let th4 = CONV_RULE(RAND_CONV(RAND_CONV WORD_VAL_CONV)) th3 in
+       let th5 = GEN_REWRITE_RULE (RAND_CONV o RAND_CONV) [NUMERAL] th4 in
+       let th6 = CONV_RULE(RAND_CONV conv) th5 in
+       PROVE_HYP th1 (SIMPLE_CHOOSE f th6)
+     | _ -> failwith "WORD_POPCOUNT_CONV");;
+
+let WORD_EVENPARITY_CONV =
+  let conv =
+    GEN_REWRITE_CONV I [word_evenparity] THENC
+    RAND_CONV WORD_POPCOUNT_CONV THENC
+    NUM_EVEN_CONV in
+  fun tm ->
+   (match tm with
+     Comb(Const("word_evenparity",_),Comb(Const("word",_),n))
+      when is_numeral n -> conv tm
+    | _ -> failwith "WORD_EVENPARITY_CONV");;
+
+let WORD_ODDPARITY_CONV =
+  let conv =
+    GEN_REWRITE_CONV I [word_oddparity] THENC
+    RAND_CONV WORD_POPCOUNT_CONV THENC
+    NUM_ODD_CONV in
+  fun tm ->
+   (match tm with
+     Comb(Const("word_oddparity",_),Comb(Const("word",_),n))
+      when is_numeral n -> conv tm
+    | _ -> failwith "WORD_ODDPARITY_CONV");;
+
+let WORD_JSHL_CONV =
+  let pth = prove
+   (`word_jshl (word(NUMERAL m):N word) (word(NUMERAL n):N word) =
+     word_shl (word(NUMERAL m):N word)
+              (val(word(NUMERAL n):N word) MOD dimindex (:N))`,
+    REWRITE_TAC[word_jshl]) in
+  GEN_REWRITE_CONV I [pth] THENC
+  RAND_CONV(BINOP2_CONV WORD_VAL_CONV (!word_SIZE_CONV) THENC
+            NUM_MOD_CONV) THENC
+  WORD_SHL_CONV;;
+
+let WORD_JSHR_CONV =
+  let pth = prove
+   (`word_jshr (word(NUMERAL m):N word) (word(NUMERAL n):N word) =
+     word_ishr (word(NUMERAL m):N word)
+               (val(word(NUMERAL n):N word) MOD dimindex (:N))`,
+    REWRITE_TAC[word_jshr]) in
+  GEN_REWRITE_CONV I [pth] THENC
+  RAND_CONV(BINOP2_CONV WORD_VAL_CONV (!word_SIZE_CONV) THENC
+            NUM_MOD_CONV) THENC
+  WORD_ISHR_CONV;;
+
+let WORD_JUSHR_CONV =
+  let pth = prove
+   (`word_jushr (word(NUMERAL m):N word) (word(NUMERAL n):N word) =
+     word_ushr (word(NUMERAL m):N word)
+               (val(word(NUMERAL n):N word) MOD dimindex (:N))`,
+    REWRITE_TAC[word_jushr]) in
+  GEN_REWRITE_CONV I [pth] THENC
+  RAND_CONV(BINOP2_CONV WORD_VAL_CONV (!word_SIZE_CONV) THENC
+            NUM_MOD_CONV) THENC
+  WORD_USHR_CONV;;
+
+let WORD_JDIV_CONV =
+  let pth = prove
+   (`word_jdiv (word(NUMERAL m):N word) (word(NUMERAL n)) =
+     (\a b. iword((int_sgn a * int_sgn b) * (abs a div abs b)))
+     (ival(word(NUMERAL m):N word)) (ival(word(NUMERAL n):N word))`,
+    REWRITE_TAC[word_jdiv; imodular; GSYM INT_MUL_ASSOC]) in
+  GEN_REWRITE_CONV I [pth] THENC
+  RATOR_CONV(RAND_CONV WORD_IVAL_CONV THENC BETA_CONV) THENC
+  RAND_CONV WORD_IVAL_CONV THENC BETA_CONV THENC
+  RAND_CONV(COMB2_CONV
+             (RAND_CONV (BINOP_CONV INT_SGN_CONV THENC INT_MUL_CONV))
+             (BINOP_CONV INT_ABS_CONV THENC INT_DIV_CONV) THENC
+            INT_MUL_CONV) THENC
+  WORD_IWORD_CONV;;
+
+let WORD_JREM_CONV =
+  let pth = prove
+   (`word_jrem (word(NUMERAL m):N word) (word(NUMERAL n):N word) =
+     word_sub (word (NUMERAL m))
+              (word_mul (word_jdiv (word (NUMERAL m)) (word (NUMERAL n)))
+                        (word (NUMERAL n)))`,
+    REWRITE_TAC[word_jrem]) in
+  GEN_REWRITE_CONV I [pth] THENC
+  RAND_CONV (LAND_CONV WORD_JDIV_CONV THENC WORD_MUL_CONV) THENC
+  WORD_SUB_CONV;;
+
+let WORD_RED_CONV =
+  let gconv_net = itlist (uncurry net_of_conv)
+   [`word(NUMERAL n):N word`,CHANGED_CONV WORD_WORD_CONV;
+    `iword i:N word`,WORD_IWORD_CONV;
+    `val(w:N word)`,WORD_VAL_CONV;
+    `ival(w:N word)`,WORD_IVAL_CONV;
+    `bit (NUMERAL k) (word(NUMERAL n):N word)`,WORD_BIT_CONV;
+    `word(NUMERAL m):N word = word(NUMERAL n)`,WORD_EQ_CONV;
+    `word_ult (word(NUMERAL m):N word) (word(NUMERAL n))`,WORD_ULT_CONV;
+    `word_ule (word(NUMERAL m):N word) (word(NUMERAL n))`,WORD_ULE_CONV;
+    `word_ugt (word(NUMERAL m):N word) (word(NUMERAL n))`,WORD_UGT_CONV;
+    `word_uge (word(NUMERAL m):N word) (word(NUMERAL n))`,WORD_UGE_CONV;
+    `word_ilt (word(NUMERAL m):N word) (word(NUMERAL n))`,WORD_ILT_CONV;
+    `word_ile (word(NUMERAL m):N word) (word(NUMERAL n))`,WORD_ILE_CONV;
+    `word_igt (word(NUMERAL m):N word) (word(NUMERAL n))`,WORD_IGT_CONV;
+    `word_ige (word(NUMERAL m):N word) (word(NUMERAL n))`,WORD_IGE_CONV;
+    `word_neg (word(NUMERAL n):N word)`,WORD_NEG_CONV;
+    `word_add (word(NUMERAL m):N word) (word(NUMERAL n))`,WORD_ADD_CONV;
+    `word_mul (word(NUMERAL m):N word) (word(NUMERAL n))`,WORD_MUL_CONV;
+    `word_sub (word(NUMERAL m):N word) (word(NUMERAL n))`,WORD_SUB_CONV;
+    `word_udiv (word(NUMERAL m):N word) (word(NUMERAL n))`,WORD_UDIV_CONV;
+    `word_umod (word(NUMERAL m):N word) (word(NUMERAL n))`,WORD_UMOD_CONV;
+    `word_umax (word(NUMERAL m):N word) (word(NUMERAL n))`,WORD_UMAX_CONV;
+    `word_umin (word(NUMERAL m):N word) (word(NUMERAL n))`,WORD_UMIN_CONV;
+    `word_imax (word(NUMERAL m):N word) (word(NUMERAL n))`,WORD_IMAX_CONV;
+    `word_imin (word(NUMERAL m):N word) (word(NUMERAL n))`,WORD_IMIN_CONV;
+    `word_shl (word(NUMERAL m):N word) (NUMERAL n)`,WORD_SHL_CONV;
+    `word_ushr (word(NUMERAL m):N word) (NUMERAL n)`,WORD_USHR_CONV;
+    `word_ishr (word(NUMERAL m):N word) (NUMERAL n)`,WORD_ISHR_CONV;
+    `word_not (word(NUMERAL n):N word)`,WORD_NOT_CONV;
+    `word_and (word(NUMERAL m):N word) (word(NUMERAL n))`,WORD_AND_CONV;
+    `word_or (word(NUMERAL m):N word) (word(NUMERAL n))`,WORD_OR_CONV;
+    `word_xor (word(NUMERAL m):N word) (word(NUMERAL n))`,WORD_XOR_CONV;
+    `word_rol (word(NUMERAL m):N word) (NUMERAL n)`,WORD_ROL_CONV;
+    `word_ror (word(NUMERAL m):N word) (NUMERAL n)`,WORD_ROR_CONV;
+    `word_zx (word(NUMERAL n):N word)`,WORD_ZX_CONV;
+    `word_sx (word(NUMERAL n):N word)`,WORD_SX_CONV;
+    `word_cand (word(NUMERAL m):N word) (word(NUMERAL n))`,WORD_CAND_CONV;
+    `word_cor (word(NUMERAL m):N word) (word(NUMERAL n))`,WORD_COR_CONV;
+    `word_join (word(NUMERAL m):M word) (word(NUMERAL n):N word)`,
+                WORD_JOIN_CONV;
+    `word_subword (word(NUMERAL m):M word) (NUMERAL p,NUMERAL q):N word`,
+                WORD_SUBWORD_CONV;
+    `bits_of_word (word(NUMERAL n):N word)`,WORD_BITS_OF_WORD_CONV;
+    `word_popcount (word(NUMERAL n):N word)`,WORD_POPCOUNT_CONV;
+    `word_evenparity (word(NUMERAL n):N word)`,WORD_EVENPARITY_CONV;
+    `word_oddparity (word(NUMERAL n):N word)`,WORD_ODDPARITY_CONV;
+    `word_jshl (word(NUMERAL m):N word) (word(NUMERAL n))`,WORD_JSHL_CONV;
+    `word_jshr (word(NUMERAL m):N word) (word(NUMERAL n))`,WORD_JSHR_CONV;
+    `word_jushr (word(NUMERAL m):N word) (word(NUMERAL n))`,WORD_JUSHR_CONV;
+    `word_jdiv (word(NUMERAL m):N word) (word(NUMERAL n))`,WORD_JDIV_CONV;
+    `word_jrem (word(NUMERAL m):N word) (word(NUMERAL n))`,WORD_JREM_CONV]
+  (basic_net()) in
+  REWRITES_CONV gconv_net;;
+
+let WORD_REDUCE_CONV = DEPTH_CONV WORD_RED_CONV;;
+
+(* ------------------------------------------------------------------------- *)
+(* Alternative returning signed words.                                       *)
+(* ------------------------------------------------------------------------- *)
+
+let WORD_TO_IWORD_CONV =
+  let pth = prove
+   (`word(NUMERAL n):N word = iword(ival(word(NUMERAL n):N word))`,
+    REWRITE_TAC[IWORD_IVAL]) in
+  GEN_REWRITE_CONV I [pth] THENC RAND_CONV WORD_IVAL_CONV;;
+
+let WORD_IREDUCE_CONV =
+  WORD_REDUCE_CONV THENC ONCE_DEPTH_CONV WORD_TO_IWORD_CONV;;
